test/test_impl.dfy
@@ -13,20 +13,11 @@ module test_impl {
     import opened test_helpers
     import opened L1_Spec
     import opened L1_CommonFunctions
-    lemma recoverSignedProposalAuthorCanEvaluateAMagicNumberToAnHonestNode()
-    {
-        var up := UnsignedProposal(0,0,0);
-        var sp := SignedProposal(up, 0); // the signature is 0
-        // nodes in the network are 0,1,2,3, where 0 is the faulty node
-        assume signProposal(up, 1).signature != 0;
-        lemmaSignedProposal();
-        assert recoverSignedProposalAuthor(sp) != 1;
-    }
 
     lemma getNewBlockCanGetValidCommitSeals()
     {
         assume forall blockchain ::validators(blockchain) == [0,1,2,3];
-        var block1 := Block(BlockHeader(0, 0, {}, 1, 0), "block1", []); // a random block with empty commit seals
+        var block1 := Block(BlockHeader(0, 0, {}, 1, 0), 1, []); // a random block with empty commit seals
         var commitSeals1 := {signHash(hashBlockForCommitSeal(block1), 1), signHash(hashBlockForCommitSeal(block1), 2), signHash(hashBlockForCommitSeal(block1), 3)}; // constructing valid commit seals from a quorum of honest nodes
         var signedBlock1 := block1.(header := block1.header.(commitSeals := commitSeals1)); // put the commit seals into the block
 
@@ -41,13 +32,9 @@ module test_impl {
         assert DSInit(s, c());
 
         // 
-        var block1 := Block(BlockHeader(0, 0, {}, 1, 0), "block1", []); // a random block with empty commit seals
+        var block1 := Block(BlockHeader(0, 0, {}, 1, 0), 1, []); // a random block with empty commit seals
         var commitSeals1 := {signHash(hashBlockForCommitSeal(block1), 1), signHash(hashBlockForCommitSeal(block1), 2), signHash(hashBlockForCommitSeal(block1), 3)}; // constructing valid commit seals from a quorum of honest nodes
         var signedBlock1 := block1.(header := block1.header.(commitSeals := commitSeals1)); // put the commit seals into the block
-
-
-
-
 
     }
 }
