doc.md
@@ -1,22 +1,2 @@
-***: potential bugs
-
 proof: instr_dsstate_multiple_invariants.dfy
 lemmaInstrDSNextMultipleIndInvForBlockchainConsistency
-
-***: adversary should also be able to send other messages (unsigned or incorrectly signed)  --  if the implementation does not check signature, the proof will still pass
-
-***: why the state of an adversary node cannot change
-
-***: adversary: proposal can be signed by adversary, but other types of message cannot?
-
-
-
-
-
-
-
-***: validDSState(s) in distributed system be a &&?
-
-
-
-***: genesisBlock is not forced to be the first block in each blockchain
